src/lowparse/LowParse.Steel.ArrayPtr.fsti
@@ -1,0 +1,291 @@
+(*
+   Copyright 2021 Microsoft Research
+
+   Licensed under the Apache License, Version 2.0 (the "License");
+   you may not use this file except in compliance with the License.
+   You may obtain a copy of the License at
+
+       http://www.apache.org/licenses/LICENSE-2.0
+
+   Unless required by applicable law or agreed to in writing, software
+   distributed under the License is distributed on an "AS IS" BASIS,
+   WITHOUT WARRANTIES OR CONDITIONS OF ANY KIND, either express or implied.
+   See the License for the specific language governing permissions and
+   limitations under the License.
+*)
+
+(* A partial model for C array pointers. Given a type t, we model type
+   t* with the following operations:
+
+   * null
+
+   * alloc, free
+
+   * read at some offset p[i]
+   
+   * additive pointer arithmetic: if p is an array pointer, then the
+     user has permission to access n cells to its right-hand-side (no
+     subtractions.) So if i <= n, then operation q = p+i splits the
+     permission into two parts, p for cells from 0 to i-1, and q for
+     cells from i to n-1. User needs to explicitly return the
+     permission by "merging" back q into p.
+*)
+
+module LowParse.Steel.ArrayPtr
+open Steel.Memory
+open Steel.Effect
+open Steel.FractionalPermission
+open Steel.Effect.Atomic
+module U32 = FStar.UInt32
+module A = Steel.Array
+
+val t (t:Type u#0) : Type u#0
+
+val g_is_null (#a: Type) (x: t a) : GTot bool
+
+val null (a: Type) : Pure (t a) (requires True) (ensures (fun res -> g_is_null res == true))
+
+val null_unique (#a: Type) (x: t a) : Lemma
+  (requires (g_is_null x == true))
+  (ensures (x == null a))
+
+[@@erasable]
+noeq type v (t: Type u#0) = {
+  array: A.array t;                      (* spatial permission range *)
+  contents: Seq.lseq t (A.length array); (* actual contents *)
+  perm: perm;                            (* temporal permission *)
+  prf: squash (A.length array < 2147483648); (* TODO: remove and switch to size_t *)
+}
+
+val is_arrayptr (#a:Type0) (r:t a) : slprop u#1
+val arrayptr_sel (#a:Type0) (r:t a) : selector (v a) (is_arrayptr r)
+
+[@@ __steel_reduce__]
+let varrayptr' #a r : vprop' =
+  {hp = is_arrayptr r;
+   t = v a;
+   sel = arrayptr_sel r}
+
+[@@ __steel_reduce__]
+let varrayptr r = VUnit (varrayptr' r)
+
+[@@ __steel_reduce__]
+let sel (#a:Type) (#p:vprop) (r:t a)
+  (h:rmem p{FStar.Tactics.with_tactic selector_tactic (can_be_split p (varrayptr r) /\ True)})
+: GTot (v a)
+  = h (varrayptr r)
+
+val varrayptr_not_null
+  (#opened: _)
+  (#a: Type)
+  (x: t a)
+: SteelGhost unit opened
+    (varrayptr x)
+    (fun _ -> varrayptr x)
+    (fun _ -> True)
+    (fun h _ h' ->
+      h' (varrayptr x) == h (varrayptr x) /\
+      g_is_null x == false
+    )
+
+
+val is_arrayptr_or_null (#a:Type0) (r:t a) : slprop u#1
+val arrayptr_or_null_sel (#a:Type0) (r:t a) : selector (option (v a)) (is_arrayptr_or_null r)
+
+[@@ __steel_reduce__]
+let varrayptr_or_null' #a r : vprop' =
+  {hp = is_arrayptr_or_null r;
+   t = option (v a);
+   sel = arrayptr_or_null_sel r}
+
+[@@ __steel_reduce__]
+let varrayptr_or_null r = VUnit (varrayptr_or_null' r)
+
+val intro_varrayptr_or_null_none
+  (#opened: _)
+  (#a: Type)
+  (x: t a)
+: SteelGhost unit opened
+    emp
+    (fun _ -> varrayptr_or_null x)
+    (fun _ -> g_is_null x == true)
+    (fun _ _ h' -> h' (varrayptr_or_null x) == None)
+
+val intro_varrayptr_or_null_some
+  (#opened: _)
+  (#a: Type)
+  (x: t a)
+: SteelGhost unit opened
+    (varrayptr x)
+    (fun _ -> varrayptr_or_null x)
+    (fun _ -> True)
+    (fun h _ h' ->
+      g_is_null x == false /\
+      h' (varrayptr_or_null x) == Some (h (varrayptr x)
+    ))
+
+val elim_varrayptr_or_null_some
+  (#opened: _)
+  (#a: Type)
+  (x: t a)
+: SteelGhost unit opened
+    (varrayptr_or_null x)
+    (fun _ -> varrayptr x)
+    (fun h -> g_is_null x == false \/ Some? (h (varrayptr_or_null x)))
+    (fun h _ h' ->
+      g_is_null x == false /\
+      h (varrayptr_or_null x) == Some (h' (varrayptr x))
+    )
+
+val elim_varrayptr_or_null_none
+  (#opened: _)
+  (#a: Type)
+  (x: t a)
+: SteelGhost unit opened
+    (varrayptr_or_null x)
+    (fun _ -> emp)
+    (fun h -> g_is_null x == true \/ None? (h (varrayptr_or_null x)))
+    (fun h _ _ ->
+      g_is_null x == true /\
+      h (varrayptr_or_null x) == None
+    )
+
+val is_null
+  (#opened: _)
+  (#a: Type)
+  (x: t a)
+: SteelAtomic bool opened
+    (varrayptr_or_null x)
+    (fun _ -> varrayptr_or_null x)
+    (fun _ -> True)
+    (fun h res h' ->
+      let s = h (varrayptr_or_null x) in
+      h' (varrayptr_or_null x) == s /\
+      res == None? s /\
+      res == g_is_null x
+    )
+
+(* Splitting an array (inspired from Steel.Array) *)
+
+val join (#opened: _) (#a:Type) (al ar:t a)
+  : SteelGhost unit opened
+          (varrayptr al `star` varrayptr ar)
+          (fun _ -> varrayptr al)
+          (fun h ->
+            A.adjacent (h (varrayptr al)).array (h (varrayptr ar)).array /\
+            (h (varrayptr al)).perm == (h (varrayptr ar)).perm
+          )
+          (fun h _ h' ->
+            let cl = h (varrayptr al) in
+            let cr = h (varrayptr ar) in
+            let c' = h' (varrayptr al) in
+            A.merge_into cl.array cr.array c'.array /\
+            c'.perm == cl.perm /\
+            c'.contents == cl.contents `Seq.append` cr.contents
+          )
+
+val split (#opened: _) (#a:Type) (x: t a) (i:U32.t)
+  : SteelAtomic (t a) opened
+          (varrayptr x)
+          (fun res -> varrayptr x `star` varrayptr res)
+          (fun h -> U32.v i <= A.length (h (varrayptr x)).array)
+          (fun h res h' ->
+            let s = h (varrayptr x) in
+            let sl = h' (varrayptr x) in
+            let sr = h' (varrayptr res) in
+            U32.v i <= A.length s.array /\
+            A.merge_into sl.array sr.array s.array /\
+            sl.perm == s.perm /\
+            sr.perm == s.perm /\
+            sl.contents == Seq.slice s.contents 0 (U32.v i) /\
+            A.length sl.array == U32.v i /\
+            A.length sr.array == A.length s.array - U32.v i /\
+            sr.contents == Seq.slice s.contents (U32.v i) (A.length s.array) /\
+            s.contents == sl.contents `Seq.append` sr.contents
+          )
+
+val alloc (#a:Type) (x:a) (n:U32.t)
+  : Steel (t a)
+             emp
+             (fun r -> varrayptr r)
+             (requires fun _ -> True)
+             (ensures fun _ r h1 ->
+               (h1 (varrayptr r)).contents == Seq.create (U32.v n) x /\
+               (h1 (varrayptr r)).perm == full_perm /\
+               A.freeable (h1 (varrayptr r)).array
+             )
+
+val index (#a:Type) (r: t a) (i:U32.t)
+  : Steel a
+             (varrayptr r)
+             (fun _ -> varrayptr r)
+             (requires fun h -> U32.v i < A.length (h (varrayptr r)).array)
+             (ensures fun h0 y h1 ->
+               let s = h0 (varrayptr r) in
+               h1 (varrayptr r) == s /\
+               U32.v i < A.length s.array /\
+               y == Seq.index s.contents (U32.v i))
+
+val upd (#a:Type) (r: t a) (i:U32.t) (x:a)
+  : Steel unit
+             (varrayptr r)
+             (fun _ -> varrayptr r)
+             (requires fun h ->
+               (h (varrayptr r)).perm == full_perm /\
+               U32.v i < A.length (h (varrayptr r)).array
+             )
+             (ensures fun h0 _ h1 ->
+               let s = h0 (varrayptr r) in
+               let s' = h1 (varrayptr r) in
+               s'.array == s.array /\
+               s'.perm == full_perm /\
+               U32.v i < A.length s.array /\
+               s'.contents == Seq.upd s.contents (U32.v i) x)
+
+val free (#a:Type) (r:t a)
+  : Steel unit
+             (varrayptr r)
+             (fun _ -> emp)
+             (requires fun h ->
+               (h (varrayptr r)).perm == full_perm /\
+               A.freeable (h (varrayptr r)).array
+             )
+             (ensures fun _ _ _ -> True)
+
+val share (#opened: _) (#a: Type) (r: t a)
+  : SteelAtomic (t a) opened
+    (varrayptr r)
+    (fun res -> varrayptr r `star` varrayptr res)
+    (fun _ -> True)
+    (fun h res h' ->
+      let s = h (varrayptr r) in
+      let d = h' (varrayptr res) in
+      let s' = h' (varrayptr r) in
+      s'.perm == half_perm s.perm /\
+      s'.array == s.array /\
+      s'.contents == s.contents /\
+      d.array == s.array /\
+      d.perm == half_perm s.perm /\
+      d.contents == s.contents
+    )
+
+val gather
+  (#opened: _)
+  (#a: Type)
+  (r1 r2: t a)
+: SteelGhost unit opened
+    (varrayptr r1 `star` varrayptr r2)
+    (fun _ -> varrayptr r1)
+    (fun h ->
+      (h (varrayptr r1)).array == (h (varrayptr r2)).array
+    )
+    (fun h res h' ->
+      let s1 = h (varrayptr r1) in
+      let s2 = h (varrayptr r2) in
+      let s' = h' (varrayptr r1) in
+      s'.array == s1.array /\
+      s'.array == s2.array /\
+      s'.contents == s1.contents /\
+      s'.contents == s2.contents /\
+      s'.perm == s1.perm `sum_perm` s2.perm
+    )
